split off deterministic trace production into own theorem

rocq/definitions/Lang.v
@@ -32,7 +32,8 @@ Module Type LangDefs.
   (* Production properties *)
   Section Production.
     (* notation for single step progression *)
-    Definition steps_to_combined cs1 a cs2 := steps_to (fst cs1) (snd cs1) a (fst cs2) (snd cs2).
+    Definition steps_to_combined cs1 a cs2 := (steps_to (fst cs1) (snd cs1) a (fst cs2) (snd cs2)).
+    Hint Unfold steps_to_combined : core.
     
     Notation "cs1 '-->[' a ']' cs2" := (steps_to_combined cs1 a cs2) (at level 50, no associativity).
 
