rocq/theories/Psni.v
@@ -46,7 +46,7 @@ Module Type PSNI (B : Basic) (BT : BaseTheories B) (LD : LangDefs) (TD : TraceDe
           + pose proof trace_pfx_production c m2 s2 as [HDtprod _].
             pose proof HDtprod Hcs2 p2; simpl in H0.
             inversion Hpfx; subst.
-            rewrite <-H0. assumption.
+            apply H0. assumption.
           + assumption.
       - destruct H1.
         assumption.
@@ -76,16 +76,16 @@ Module Type PSNI (B : Basic) (BT : BaseTheories B) (LD : LangDefs) (TD : TraceDe
       unfold HPsniD, KPsniD.
       intros c HHPsniD p m a ? ?.
       pose proof trace_pfx_production as Htraceprod.
-      pose proof (hpsni_memset_invariance c HHPsniD m) as Htmp.
+      pose proof (hpsni_memset_invariance c HHPsniD m) as Hinv.
       assert (Same_set Store (atk_knowledge c m p) (indistincts c m)). {
         apply (prefix_prefix_prod p (p ++ [a]) (app_prefix a p)) in H.
         apply (trace_max c m p) in H as [st [Hepfx Htprod]]. 
-        apply Htmp with st; assumption.
+        apply Hinv with st; assumption.
       }
       assert (Same_set Store (indistincts c m) (atk_knowledge c m (p ++ [a]))). {
         apply (trace_max c m (p ++ [a])) in H as [st [Hepfx Htprod]].
         apply Same_set_sym.
-        apply Htmp with st; assumption.
+        apply Hinv with st; assumption.
       }
       apply Same_set_trans with (indistincts c m); assumption.
     Qed.
@@ -145,8 +145,8 @@ Module Type PSNI (B : Basic) (BT : BaseTheories B) (LD : LangDefs) (TD : TraceDe
       pose proof trace_max c m2 p2 Hp2prod as [stp2 [Hp2pfx Ht2prod]].
       exists (m2, p2).
       split.
-      - rewrite (trace_pfx_production c m2 st2) in H0.
-        rewrite <-H0 in Hp2prod.
+      - pose proof det_trace_pfx_production one_step_det c m2 st2 H0 p2.
+        apply H1.
         assumption.
       - unfold deq_pfx.
         eauto.
