rocq/theories/TraceTheories.v
@@ -7,8 +7,7 @@ Module Type TraceTheories (B : Basic) (LD : LangDefs) (TD : TraceDefs B LD).
   Import LangNotations.
 
   (* defn: to produce a trace means producing all finite prefixes of it *)
-  (* addn from determinism: if a trace prefix is produced by the program, then it must be a prefix of the list *)
-  Axiom trace_pfx_production : forall c m st, c ~~> (m, st) <-> (forall p, (m, p) <=| (m, st) <-> (c, m) ==>*[p]).
+  Axiom trace_pfx_production : forall c m st, c ~~> (m, st) <-> (forall p, (m, p) <=| (m, st) -> (c, m) ==>*[p]).
   (* any finite trace prefix can be expanded to an infinite trace *)
   Axiom trace_max : forall c m p, (c, m)==>*[p] -> exists (t : EvtStream), (m, p) <=| (m, t) /\ c ~~>(m, t).
   (* all configurations produce a trace *)
@@ -72,83 +71,6 @@ Module Type TraceTheories (B : Basic) (LD : LangDefs) (TD : TraceDefs B LD).
   Ltac handle_prog_contradict :=
     lazymatch goal with
       | [H : (~ (can_step ?c ?s)), H1 : (steps_to ?c ?s ?e ?c' ?s') |- _] => apply produce_impl_canstep in H1; contradiction
+      | [H : steps_to_combined _ _ _ |- _] => unfold steps_to_combined in H; handle_prog_contradict
     end.
-
-  (* note: below theories are conditioned on determinism used in subst_eq_steps *)
-  (* 
-  Lemma deterministic_step : forall cs cs1 a1,
-        cs -->[a1] cs1 -> forall cs2 a2, cs -->[a2] cs2 -> cs1 = cs2 /\ a1 = a2.
-      intros cs cs1 a1 Step1 ? ? ?.
-      pose proof (deterministic cs cs1 cs2 a1 a2).
-      apply H0; assumption.
-  Qed.
-  Ltac subst_eq_steps :=
-    repeat lazymatch goal with
-      | [H : (_, _) = (_, _) |- _] => injection H ; intros ; subst ; clear H
-      | [H0 : ?cs -->[?a0] ?cs0, H1 : ?cs -->[?a1] ?cs1 |- _]
-        => assert (cs1 = cs0 /\ a1 = a0) as [? ?] by eauto using deterministic_step ; subst ; clear H1 
-    end.
-
-  Lemma evt_prefix_prod_both : forall lst st0, EvtPrefix lst st0 -> forall c s st1, Produces c s st0 -> Produces c s st1 -> EvtPrefix lst st1.
-    intros lst st0 EvtPfx. induction EvtPfx ; intros c s st1 Prod0 Prod1 ; auto using EvtPrefix_empty.
-    inversion Prod0 ; inversion Prod1 ; subst; subst_eq_steps.
-    - eauto using EvtPrefix_some.
-    - handle_prog_contradict.
-  Qed.
-
-  Lemma pfx_prod_both : forall pfx s st0, pfx <=| (s, st0) -> forall c st1, Produces c s st0 -> Produces c s st1 -> pfx <=| (s, st1).
-    intros pfx s st0 PfxOf0 c st1 Prod0 Prod1.
-    inversion PfxOf0 as [? lst ? EvtPfx]. subst.
-    eauto using LeTrace_intro, evt_prefix_prod_both.
-  Qed.
-
-  Lemma prod_mstep : forall c s cs lst, (c, s) ==>*[lst] cs -> forall st, Produces c s st
-      -> exists st', Produces c s (prepend lst st').
-    intros c s cs lst MStep. dependent induction MStep ; intros st Prod ; eauto.
-    destruct cs1 as [c1 s1].
-    inversion Prod ; subst.
-    - subst_eq_steps.
-      assert (exists st', Produces c1 s1 (prepend lst st')) as [st' ?] by eauto.
-      eauto using Produces_step.
-    - handle_prog_contradict.
-  Qed. 
-
-  Lemma prod_prepend_mstep : forall c s c' s' lst, (c, s) ==>*[lst] (c', s')
-      -> forall st, Produces c s (prepend lst st) -> Produces c' s' st.
-    intros c s c' s' lst MStep. dependent induction MStep ; intros st ProdPrepend ; auto.
-    destruct cs1 as [c1 s1].
-    simpl in ProdPrepend ; inversion ProdPrepend ; subst ; subst_eq_steps.
-    eauto.
-  Qed. 
-
-  Lemma prod_prefix_mstep : forall lst c s st, Produces c s st
-      -> EvtPrefix lst st
-      -> exists cs, (c, s) ==>*[lst] cs.
-    induction lst ; intros c s st Prod Pfx ; eauto using MultiStep_refl.
-    inversion Pfx ; subst.
-    inversion Prod ; subst.
-    assert (exists cs, (c', s') ==>*[lst] cs) as [? ?] by eauto.
-    eauto using MultiStep.
-  Qed.
-
-  Lemma prod_mstep_prefix : forall lst c s st cs, Produces c s st
-      -> (c, s) ==>*[lst] cs
-      -> EvtPrefix lst st.
-    induction lst ; intros c s st cs Prod MStep ; eauto using EvtPrefix_empty.
-    inversion MStep ; subst ; inversion Prod ; subst.
-    - destruct cs1 as [c1 s1] ; subst_eq_steps.
-      eauto using EvtPrefix_some.
-    - handle_prog_contradict.
-  Qed.
-
-  Lemma prod_conv_prefix : forall lst st, EvtPrefix lst st
-      -> forall c s c' s' lst', (c, s) ==>*[lst'] (c', s') /\ ~ can_step c' s'
-      -> Produces c s st
-      -> Prefix lst lst'.
-      intros lst st EvtPfx. induction EvtPfx ; intros c s c' s' lst' Conv Prod ; auto.
-      inversion Prod; subst; destruct Conv as [Conv Hend]; inversion Conv; subst.
-      - handle_prog_contradict.
-      - subst_eq_steps.
-        eauto.
-  Qed. *)
 End TraceTheories.
